src/Oeuf.v
@@ -1,4 +1,4 @@
-Require Import compcert.driver.Compiler compcert.common.Errors.
+Require Import OeufCompcertCompiler compcert.common.Errors.
 Require Import Common Monads.
 Require UntypedComp TaggedComp LiftedComp SwitchedComp FmajorComp.
 Require Fmajortofflatmajor Fflatmajortoemajor Emajortodmajor Dflatmajortocmajor Cmajortominor.
